@prefix owl: <http://www.w3.org/2002/07/owl#> .
@prefix xsd: <http://www.w3.org/2001/XMLSchema#> .
@prefix dct: <http://purl.org/dc/terms/> .
@prefix rdf: <http://www.w3.org/1999/02/22-rdf-syntax-ns#> .
@prefix rdfs: <http://www.w3.org/2000/01/rdf-schema#> .
@prefix skos: <http://www.w3.org/2004/02/skos/core#> .
@prefix xl: <http://www.w3.org/2008/05/skos-xl#> .
@predix atifrax: <http://uri.tbd/atifrax#> .

#####
# This schema formalizes a set of semantic conditions sufficient to model 
# artifacts for use and/or reuse in RPGs. 
#####


# Ontology

atifrax: a owl:Ontology ;
  dct:title "atifrax schema"@en ;
  dct:description "A schema for modeling artifacts for use and/or reuse in RPGs." .


# OWL Classes

atifrax:Fractus a owl:Class ;
  rdfs:label "Fractus"@en ;
  skos:definition "A collection of Artifact instances collected under one designation."@en ;
  skos:scopeNote "A fractus may be defined to include artifcats from different sources."@en ;
  owl:disjointWith atifrax:Artifact .

atifrax:Artifact a owl:Class ;
  rdfs:label "Artifact"@en ;
  skos:definition "A collection of Mechanics, Flavors, and Artworks. Each Artifact is a compound class."@en ;
  skos:scopeNote "An artifact may be defined to include mechanics, flavors, and artworks from different sources. Each will be attributed and licensed appropriately."@en ;
  owl:disjointWith atifrax:Fractus .

atifrax:Constituent a owl:Class ;
  rdfs:label "Constituent"@en ;
  skos:definition "Superclass of components that can be included with an artifact."@en ;
  skos:scopeNote "This class is not intended to be used directly, but as a superclass for all classes that an artifact may include."@en ;
  owl:disjointWith atifrax:Artifact , atifrax:Fractus .

atifrax:Mechanic a owl:Class ;
  rdfs:label "Mechanic"@en ;
  skos:definition "Superclass of all materials involving game rules, parameters, and specifications that are mechanical or computational in nature."@en ;
  skos:scopeNote "Mechanics must be defined as granularly as possible, preferably comprising only a single rule or computation."@en ;
  rdfs:subClassOf atifrax:ArtifactConstituent ;
  owl:disjointWith atifrax:Flavor , atifrax:Artwork .

atifrax:Flavor a owl:Class ;
  rdfs:label "Flavor"@en ;
  skos:definition "Superclass of all materials involving descriptive text that are not mechanical or computational in nature and are not otherwise artworks. Examples include setting descriptions, names of cities, etc."@en ;
  skos:scopeNote "Flavors MUST NOT be defined to impose rules or mechanics." ;
  rdfs:subClassOf atifrax:ArtifactConstituent ;
  owl:disjointWith atifrax:Mechanic , atifrax:Artwork .

atifrax:Artwork a owl:Class ;
  rdfs:label "Artwork"@en ;
  skos:definition "Superclass of all materials involving primarily artistic works distinct from flavor text and not mechanical or computational in nature."
  skos:scopeNote "Artworks MUST NOT be defined to impose rules or mechanics." ;
  rdfs:subClassOf atifrax:ArtifactConstituent ;
  owl:disjointWith atifrax:Mechanic , atifrax:Flavor .


# DatatypeProperties
# TO DO: define data properties; 

# ObjectProperties

atifrax:hasArtifact a rdfs:Property , owl:ObjectProperty ;
  rdfs:label "has artifact"@en ;
  skos:definition "Relates a fractus to constituent artifacts."@en ;
  rdfs:comment "Generally speaking, artifacts do not assert their inclusion in a fractus; it is up to the fractus to declare its constituent parts."@en ;
  rdfs:domain atifrax:Fractus ;
  rdfs:range atifrax:Artifact .

atifrax:hasConstituent a rdfs:Property , owl:ObjectProperty ;
  rdfs:label "has constituent"@en ;
  skos:definition "Relates an artifact to its constituent parts."@en ;
  rdfs:comment "Generally, constituents do not assert their inclusion in an artifact; it is up to the artifact to declare its constituent parts."@en ;
  rdfs:domain atifrax:Artifact ;
  rdfs:range atifrax:Constituent .
